\begin{frame}
\vskip -0.15cm
\begin{example}

Solve the polynomial system.
$
\left| 
\begin{array}{rcl}
\alertNoH{26,29}{ x-\alertNoH{2}{4y}}&\alertNoH{26,29}{{=}}&\alertNoH{26,29}{5}\\
\alertNoH{26,29}{\alertNoH{3}{y^2+xy}}&\alertNoH{3,26,29}{{=}}&\alertNoH{3,26,29}{10}
\end{array}
\right.
$

\only<handout:1|1-22>{
\hfil\hfil$\begin{array}{rcl@{}l@{}|l}
\uncover<2->{\alertNoH{4,14,17}{ x} &\alertNoH{4,14,17}{{ =}}&\alertNoH{4, 14, 17 }{5+\alertNoH{2}{4y}} &&\text{Solve for }x \text{ in first eq-n.}} \\
\uncover<3->{\alertNoH{3}{ y^2+xy}&\alertNoH{3}{{=}}&\alertNoH{3}{10}&& \uncover<4->{\text{Substitute } x \text{ away}}}\\
\uncover<4->{y^2+\alertNoH{5}{ (\alertNoH{4}{5+4y})y}&=& \alertNoH{6}{10}}\\
\uncover<5->{\alertNoH{7}{y^2}+ \alertNoH{5}{5y+\alertNoH{7}{4y^2} }-\alertNoH{6}{10}&=&0}\\
\uncover<7->{\alertNoH{7}{\alertNoH{8,9}{5}y^2}+\alertNoH{8,9}{5}y-\alertNoH{8,9}{10}&=&0 \uncover<8->{&& \text{Divide by }\alertNoH{8,9}{5}}}\\
\uncover<9->{\alertNoH{10,11}{ y^2+y-2}&=&0}\\
\uncover<10->{(\fcAnswer{11}{ \alertNoH{12}{y+2}})(\fcAnswer{11}{\alertNoH{13}{y-1} })&=&0} \\
\uncover<12->{ \alertNoH{12,15,20}{y=-2} &\text{or} & \alertNoH{13,18,21}{y=1}}\\
\begin{array}{@{}r@{~}c@{~}l@{}} 
\uncover<14->{ \alertNoH{14,20}{x}&\alertNoH{14}{{=}}&\alertNoH{14}{5+4y}}\\
\uncover<15->{&=&\alertNoH{16}{ 5+4(\alertNoH{15}{-2})}} \uncover<16->{\alertNoH{16,20}{=-3}}
\end{array}
&& 
\begin{array}{@{}r@{~}c@{~}l@{}} 
\uncover<17->{\alertNoH{17,21}{ x}&\alertNoH{17}{{=}}&\alertNoH{17}{5+ 4\alertNoH{18}{y}}}\\
\uncover<18->{&=&\alertNoH{19}{ 5+4\cdot\alertNoH{18}{ 1}}} \uncover<19->{\alertNoH{19,21}{=9}}
\end{array}
\end{array}
$

}
\uncover<20->{\alertNoH{22,23}{ Final answer: $\alertNoH{20}{x=-3, y=-2}$ or $\alertNoH{21}{x=9,y=1}$.}}

\only<handout:2|23->{
\medskip
\uncover<24->{Check answer $\alertNoH{25}{x=-3,y=-2}$: }

\[
\left| 
\begin{array}{rclcl}
\uncover<24->{\alertNoH{26}{ \alertNoH{25}{ x}-4\alertNoH{25}{y}} }\uncover<25->{&=&(\alertNoH{25}{-3})- 4(\alertNoH{25}{-2} ) &\alertNoH{26}{=}&\alertNoH{26}{ 5}}\\
\uncover<24->{ \alertNoH{26}{ {\alertNoH{25}{y}}^2+{ \alertNoH{25}{x }}{\alertNoH{25}{y}}}} \uncover<25->{&=&( \alertNoH{25}{-2} )^2+(\alertNoH{25 }{-3})(\alertNoH{25}{-2})&\alertNoH{26}{=}&\alertNoH{26}{10}}
\end{array}
\right.
\] 

\medskip
Check answer $\alertNoH{28}{y=1, x=9} $: 

\[
\left| 
\begin{array}{rclcl}
\uncover<27->{\alertNoH{29}{\alertNoH{28}{x}-4{\alertNoH{28}{y}}}}\uncover<28->{&=& \alertNoH{28}{ 9} -4\cdot \alertNoH{28}{1}&\alertNoH{29}{ =}&\alertNoH{29}{ 5}}\\
\uncover<27->{\alertNoH{29}{{\alertNoH{28}{y}}^2+\alertNoH{28}{x}{\alertNoH{28}{y}}}} \uncover<28->{&=&{\alertNoH{28}{1}}^2+\alertNoH{28}{9}\cdot \alertNoH{28}{1} &\alertNoH{29}{=}&\alertNoH{29}{10}.}
\end{array}
\right.
\]
}
\end{example}
\vskip 10cm
\end{frame}