% begin module exponential-equation-quadratic-arbitrary-base-2
\begin{frame}
\begin{example}[Exponential equation that reduces to quadratic]
Solve the equation.
\[
\begin{array}{rcll|l}
\displaystyle 3^{2x} & =&\displaystyle \alertNoH{2}{ 2 + 63\cdot 3^{-2x}} \uncover<2->{&& \begin{array}{l} >2\text{ terms}\Rightarrow\\ 
 \text{transfer one side} \end{array}} \\
\uncover<2->{ \alertNoH{3,8,20}{3^{2x}} \alertNoH{2}{- 2 - 63\cdot \alertNoH{4,5,9}{3^{-2x}}} & = &0\uncover<3->{&& 
\begin{array}{@{}r@{~}c@{~}l} 
\alertNoH{3,7,8,20}{ 3^{2x}}&\alertNoH{3,7,8,20}{=}&\alertNoH{3,7,8,20}{u}\\
\uncover<4->{\alertNoH{4,5,9}{3^{\alertNoH{6}{-}2x}}&\alertNoH{4,5,9}{=}& \fcAnswer{5}{ \left(\alertNoH{7}{3^{2x}}\right)^{\alertNoH{6}{-1}}\uncover<7->{={\alertNoH{7,9}{u}}^{-1}}}}
\end{array}}}
\\
\uncover<8->{\displaystyle \alertNoH{8,10}{ u}-\alertNoH{11}{2}-\alertNoH{12}{63 \alertNoH{9}{u^{-1}}} &=&0\uncover<10->{ &&\text{Multiply }\alertNoH{10,11,12}{ \cdot u}}}\\
\uncover<10->{\displaystyle \alertNoH{13,14}{ \alertNoH{10}{ u^2} -\alertNoH{11}{2u}- \alertNoH{12}{ 63}}&=&0}\\
\uncover<13->{ \displaystyle (\fcAnswer{14}{\alertNoH{15}{u-9}}) (\fcAnswer{14}{\alertNoH{16}{u +7}})&=&0}\\
\uncover<15->{\displaystyle \alertNoH{15}{ u\alertNoH{19}{-9}=0}&\text{or} &\displaystyle  \alertNoH{16}{u+\alertNoH{17}{7}=0}}\\
\uncover<17->{ \displaystyle \uncover<19->{\alertNoH{20}{u}=\alertNoH{19}{ 9} }&\text{or}&  u=\alertNoH{17}{-7}}\\
\uncover<18->{\displaystyle \uncover<20->{\alertNoH{20}{3^{2x}}=9}&\text{or} &  \alertNoH{18}{\text{no real solution}}}\\
\uncover<21->{\displaystyle 2x=\alertNoH{22,23}{\log_{3} 9}} \\
\uncover<22->{\displaystyle \alertNoH{24}{2}x=\fcAnswer{23}{\alertNoH{24}{2}}}\\
\uncover<24->{\alertNoH{25}{ \displaystyle x=\alertNoH{24}{1}}}
\end{array}
\]

\end{example}
\end{frame}
% end module exponential-equation-quadratic-arbitrary-base-2
